AbsInterp.lean
@@ -38,6 +38,7 @@ import AbsInterp.Instances
 import AbsInterp.Instances.LTS
 import AbsInterp.Instances.LTS.Analyses.Common
 import AbsInterp.Instances.LTS.Analyses.Interval
+import AbsInterp.Instances.LTS.Analyses.Parity
 import AbsInterp.Instances.LTS.Analyses.Sign
 import AbsInterp.Instances.LTS.Core
 import AbsInterp.Instances.LTS.Instantiation.Interface
